trivial

src/FcEtt/ext_weak.v
@@ -191,78 +191,52 @@ Proof.
     constructor; auto 1.
     sfirstorder use:weakening_helper_propwff.
     sfirstorder use:weakening_helper_propwff.
+  (* Impl: won't go through because Impl's introduction rule is existential *)
   - admit.
 Admitted.    
-    
-    
-
- E_pick_fresh y; try auto_rew_env; apply_first_hyp; try simpl_env; eauto 3.
-  constructor; auto.
-  apply H0.
-    
-    all: try solve [E_pick_fresh y; try auto_rew_env; apply_first_hyp; try simpl_env; eauto 3].
-    simpl_env.
-  (*
-  eapply E_LeftRel with (b:=b)(b':=b'); eauto 2;
-    try eapply DefEq_weaken_available; eauto 2.
-  eapply E_LeftIrrel with (b:=b)(b':=b'); eauto 2;
-    try eapply DefEq_weaken_available; eauto 2.
-  eapply E_Right with (a:=a)(a':=a'); eauto 2;
-    try eapply DefEq_weaken_available; eauto 2.
-  *)
-Qed.
 
 
-Definition Typing_weakening  := first  typing_weakening_mutual.
-Definition PropWff_weakening := second typing_weakening_mutual.
-Definition Iso_weakening     := third  typing_weakening_mutual.
-Definition DefEq_weakening   := fourth typing_weakening_mutual.
-Definition Ctx_weakening     := fifth  typing_weakening_mutual.
+
+Lemma Typing_weakening : ∀ (E F G: context) psi (a A : tm),  Typing (F ++ G) psi a A →  Ctx (F ++ E ++ G) ->
+                                                          Typing (F ++ E ++ G) psi a A.
+Proof. sfirstorder use:typing_weakening_mutual. Qed.
 
 
-(*
-Lemma Typing_weakening : ∀ (E F G : context) (a A : tm),  Typing (F ++ G) a A →  Ctx (F ++ E ++ G) ->
-                                                          Typing (F ++ E ++ G) a A.
-Proof. intros. apply (first typing_weakening_mutual) with (G0 := F ++ G)(F:=F)(E:=E)(G:=G); auto. Qed.
+Lemma PropWff_weakening : forall (E F G : context) psi phi, PropWff (F ++ G) psi phi -> Ctx (F ++ E ++ G) → PropWff (F ++ E ++ G) psi phi.
+Proof. sfirstorder use:typing_weakening_mutual. Qed.
+
+Lemma Iso_weakening : ∀ (E F G : context) psi (p1 p2 : constraint),
+       Iso (F ++ G) psi p1 p2 -> Ctx (F ++ E ++ G) → Iso (F ++ E ++ G) psi p1 p2.
+Proof. sfirstorder use:typing_weakening_mutual. Qed.
+
+Lemma DefEq_weakening : ∀ (E F G : context) psi phi,
+    DefEq (F ++ G) psi phi → Ctx (F ++ E ++ G) → DefEq (F ++ E ++ G) psi phi.
+Proof. sfirstorder use:typing_weakening_mutual. Qed.
+
+(* I don't think anyone would want this *)
+(* Lemma Ctx_weakening : ∀ (E F G: context), *)
+(*        Ctx (F ++ G) → Ctx (F ++ E ++ G) → Ctx (F ++ E ++ G). *)
+(* Proof. intros. apply (fifth typing_weakening_mutual) with (G0 := F ++ G)(F:=F)(E:=E)(G:=G); auto. Qed. *)
 
 
-Lemma PropWff_weakening : forall (E F G : context) phi, PropWff (F ++ G) phi -> Ctx (F ++ E ++ G) → PropWff (F ++ E ++ G) phi.
-Proof. intros. apply (second typing_weakening_mutual) with (G0 := F ++ G)(F:=F)(E:=E)(G:=G); auto. Qed.
+(* subsumed by the meet_ctx_l lemmas? *)
+(* Lemma Iso_weakening_dom : *)
+(*    ∀ (E F G : context) (D : available_props) (p1 p2 : constraint), *)
+(*        Iso (F ++ G) (dom (F ++ G)) p1 p2 -> Ctx (F ++ E ++ G) → Iso (F ++ E ++ G) (dom(F ++ E ++ G)) p1 p2. *)
+(* Proof. *)
+(*   intros. *)
+(*   eapply Iso_weaken_available. *)
+(*   eapply Iso_weakening. *)
+(*   eassumption. *)
+(*   auto. *)
+(* Qed. *)
 
-Lemma Iso_weakening : ∀ (E F G : context) (D : available_props) (p1 p2 : constraint),
-       Iso (F ++ G) D p1 p2 -> Ctx (F ++ E ++ G) → Iso (F ++ E ++ G) D p1 p2.
-Proof. intros. apply (third typing_weakening_mutual) with (G0 := F ++ G)(F:=F)(E:=E)(G:=G); auto. Qed.
-
-Lemma DefEq_weakening : ∀ (E F G : context) (D : available_props) (A B T : tm),
-    DefEq (F ++ G) D A B T → Ctx (F ++ E ++ G) → DefEq (F ++ E ++ G) D A B T.
-Proof. intros. apply (fourth typing_weakening_mutual) with (G0 := F ++ G)(F:=F)(E:=E)(G:=G); auto. Qed.
-
-Lemma Ctx_weakening : ∀ (E F G: context),
-       Ctx (F ++ G) → Ctx (F ++ E ++ G) → Ctx (F ++ E ++ G).
-Proof. intros. apply (fifth typing_weakening_mutual) with (G0 := F ++ G)(F:=F)(E:=E)(G:=G); auto. Qed.
-
-
-Lemma Iso_weakening_dom :
-   ∀ (E F G : context) (D : available_props) (p1 p2 : constraint),
-       Iso (F ++ G) (dom (F ++ G)) p1 p2 -> Ctx (F ++ E ++ G) → Iso (F ++ E ++ G) (dom(F ++ E ++ G)) p1 p2.
-Proof.
-  intros.
-  eapply Iso_weaken_available.
-  eapply Iso_weakening.
-  eassumption.
-  auto.
-Qed.
-
-Lemma DefEq_weakening_dom : ∀ (E F G : context) (D : available_props) (A B T : tm),
-    DefEq (F ++ G) (dom (F ++ G)) A B T → Ctx (F ++ E ++ G) → DefEq (F ++ E ++ G) (dom (F ++ E ++ G)) A B T.
-Proof.
-  intros.
-  eapply DefEq_weaken_available.
-  eapply DefEq_weakening.
-  eassumption.
-  auto.
-Qed.
-*)
-
-
-End ext_weak.
+(* Lemma DefEq_weakening_dom : ∀ (E F G : context) (D : available_props) (A B T : tm), *)
+(*     DefEq (F ++ G) (dom (F ++ G)) A B T → Ctx (F ++ E ++ G) → DefEq (F ++ E ++ G) (dom (F ++ E ++ G)) A B T. *)
+(* Proof. *)
+(*   intros. *)
+(*   eapply DefEq_weaken_available. *)
+(*   eapply DefEq_weakening. *)
+(*   eassumption. *)
+(*   auto. *)
+(* Qed. *)
